\begin{CajaTitulo}{\begin{center}\subsection{Soluci√≥n P10}\end{center}}
    \vspace{0.5cm}
    \begin{align*}
        \int_{0}^{\infty} \frac{x}{\sinh(x)}dx &= 2\int_{0}^{\infty} \frac{x}{e^x - e^{-x}}dx\\
        &= 2\int_{0}^{\infty} \frac{x}{e^x - e^{-x}}dx\cdot \frac{e^{-x}}{e^{-x}}\\
        &= 2\int_{0}^{\infty} \frac{xe^{-x}}{1 - (e^{-x})^2}dx \: \hspace{0.3cm}\cambio{\ln(u) = -x}{du = -e^{-x}dx}\\
        &= -2\int_{0}^{1} \frac{\ln(u)}{1 - u^2}du = -2\sum_{n=1}^{\infty}\int_{0}^{1}u^{2n}\ln(u)du \: \cambio{\ln(u) = -x}{u = -e^{-x}dx} \\
        &= -2\sum_{n=1}^{\infty}\int_{0}^{1}u^{2n}\ln(u)du = -2\sum_{n=1}^{\infty}\int_{0}^{1}u^{2n}\ln(u)du \: \: \cambio{-\ln(u) = x}{du = -e^{-x}dx}\\
        &= 2\sum_{n=1}^{\infty}\int_{0}^{\infty}e^{-(2n+1)x}xdx \: \cambio{x = \frac{t}{2n+1} \vspace{0.2cm}}{dx = \frac{dt}{2n+1}}\\
        &= 2\sum_{n=1}^{\infty}\int_{0}^{\infty}\frac{t\:e^{-t}}{{(2n+1)}^2}dt = 2\sum_{n=1}^{\infty}\frac{1}{{(2n+1)}^2} = \frac{\pi^2}{4}
    \end{align*}
\end{CajaTitulo}